% Copyright (c) 2001-2011
%       H. Turgut Uyar <uyar@itu.edu.tr>
%       Ayşegül Gençata Yayımlı <gencata@itu.edu.tr>
%       Emre Harmancı <harmanci@itu.edu.tr>
%
% These notes are licensed using the
% "Creative Commons Attribution-NonCommercial-ShareAlike License".
% You are free to copy, distribute and transmit the work, and to adapt the work
% as long as you attribute the authors, do not use it for commercial purposes,
% and any derivative work is under the same or a similar license.
%
% Read the full legal code at:
% http://creativecommons.org/licenses/by-nc-sa/3.0/

\documentclass[dvipsnames]{beamer}

\usepackage{ae}
\usepackage[T1]{fontenc}
\usepackage[utf8]{inputenc}
\setbeamertemplate{navigation symbols}{}

\mode<presentation>
{
  \usetheme{Rochester}
  \setbeamercovered{transparent}
}

\title{Discrete Mathematics}
\subtitle{Propositions}

\author{H. Turgut Uyar \and Ayşegül Gençata Yayımlı \and Emre Harmancı}
\date{2001-2011}

\AtBeginSubsection[]
{
  \begin{frame}<beamer>
    \frametitle{Topics}
    \tableofcontents[currentsection,currentsubsection]
  \end{frame}
}

%\beamerdefaultoverlayspecification{<+->}

\pgfdeclareimage[width=2cm]{license}{../../license}

\begin{document}

\begin{frame}
  \titlepage
\end{frame}

\begin{frame}
  \frametitle{Licence}

  \pgfuseimage{license}\hfill
  \copyright 2001-2011 T. Uyar, A. Yayımlı, E. Harmancı

  \vfill
  \begin{tiny}
    You are free:
    \begin{itemize}
      \item to Share — to copy, distribute and transmit the work
      \item to Remix — to adapt the work
    \end{itemize}

    Under the following conditions:
    \begin{itemize}
      \item Attribution — You must attribute the work in the manner specified by
        the author or licensor (but not in any way that suggests that they
        endorse you or your use of the work).

      \item Noncommercial — You may not use this work for commercial purposes.

      \item Share Alike — If you alter, transform, or build upon this work, you
        may distribute the resulting work only under the same or similar license
        to this one.
    \end{itemize}
  \end{tiny}

  \vfill
  Legal code (the full license):\\
  \url{http://creativecommons.org/licenses/by-nc-sa/3.0/}
\end{frame}

\begin{frame}
  \frametitle{Topics}
  \tableofcontents
\end{frame}

\section{Propositions}

\subsection{Introduction}

\begin{frame}
  \frametitle{Proposition}

  \begin{definition}
    \alert{proposition} (or \alert{statement}):\\
      a declarative sentence that is either true or false
  \end{definition}

  \pause
  \begin{itemize}
    \item \alert{law of the excluded middle}:\\
      a proposition cannot be partially true or partially false
  \end{itemize}

  \pause
  \begin{itemize}
    \item \alert{law of contradiction}:\\
      a proposition cannot be both true and false
  \end{itemize}
\end{frame}

\begin{frame}
  \frametitle{Proposition Examples}

  \begin{columns}[t]
    \column{.55\textwidth}
    \begin{example}[proposition]
      \begin{itemize}
        \item The Moon revolves around the Earth.
        \item Elephants can fly.
        \item $3+8=11$
      \end{itemize}
    \end{example}

    \pause
    \column{.45\textwidth}
    \begin{example}[not a proposition]
      \begin{itemize}
        \item What time is it?
        \item Ali, throw the ball!
        \item $x<43$
      \end{itemize}
    \end{example}
  \end{columns}
\end{frame}

\begin{frame}
  \frametitle{Proposition Variable}

  \begin{definition}
    \alert{proposition variable}:\\
      a name that represents the proposition

    \begin{itemize}
      \item can take on the values \emph {True} ($T$) or \emph{False} ($F$)
    \end{itemize}
  \end{definition}

  \pause
  \begin{example}
    \begin{itemize}
      \item $p_1$: The Moon revolves around the Earth. ($T$)
      \item $p_2$: Elephants can fly. ($F$)
      \item $p_3$: $3+8=11$ ($T$)
    \end{itemize}
  \end{example}
\end{frame}

\subsection{Operations}

\begin{frame}
  \frametitle{Operations}

  \begin{itemize}
    \item new propositions can be formed by:
    \begin{itemize}
      \item negating a proposition
      \item combining two or more propositions into\\
        \alert{compound propositions} using \alert{logical connectives}
    \end{itemize}
    \item \alert{primitive propositions} can not be decomposed into smaller
      units
  \end{itemize}

  \pause
  \begin{itemize}
    \item \alert{truth table}:\\
      a table that gives the truth value of the compound proposition for all
      possible values of its primitive propositions
  \end{itemize}
\end{frame}

\begin{frame}
  \frametitle{Negation (NOT)}

  \begin{columns}
    \column{.3\textwidth}
    \begin{table}
      \caption{$\neg p$}
      \begin{tabular}{|c||c|}\hline
        $p$ & $\neg p$\\\hline\hline
        $T$ & $F$     \\\hline
        $F$ & $T$     \\\hline
      \end{tabular}
    \end{table}

    \pause
    \column{.7\textwidth}
    \begin{example}
      \begin{itemize}
        \item $\neg p_1$: The Moon does not revolve around the Earth.\\
          $\neg T$: \emph{False}
        \item $\neg p_2$: Elephants cannot fly.\\
          $\neg F$: \emph{True}
      \end{itemize}
    \end{example}
  \end{columns}
\end{frame}

\begin{frame}
  \frametitle{Conjunction (AND)}

  \begin{columns}
    \column{.4\textwidth}
    \begin{table}
      \caption{$p \wedge q$}
      \begin{tabular}{|c|c||c|}\hline
        $p$ & $q$ & $p \wedge q$\\\hline\hline
        $T$ & $T$ & $T$         \\\hline
        $T$ & $F$ & $F$         \\\hline
        $F$ & $T$ & $F$         \\\hline
        $F$ & $F$ & $F$         \\\hline
      \end{tabular}
    \end{table}

    \pause
    \column{.6\textwidth}
    \begin{example}
      \begin{itemize}
        \item $p_1 \wedge p_2$: The Moon revolves around the Earth and elephants
          can fly.\\
          $T \wedge F$: \emph{False}
      \end{itemize}
    \end{example}
  \end{columns}
\end{frame}

\begin{frame}
  \frametitle{Disjunction (OR)}

  \begin{columns}
    \column{.4\textwidth}
    \begin{table}
      \caption{$p \vee q$}
      \begin{tabular}{|c|c||c|}\hline
        $p$ & $q$ & $p \vee q$\\\hline\hline
        $T$ & $T$ & $T$       \\\hline
        $T$ & $F$ & $T$       \\\hline
        $F$ & $T$ & $T$       \\\hline
        $F$ & $F$ & $F$       \\\hline
      \end{tabular}
    \end{table}

    \pause
    \column{.6\textwidth}
    \begin{example}
      \begin{itemize}
        \item $p_1 \vee p_2$: The Moon revolves around the Earth or elephants
          can fly.\\
          $T \vee F$: \emph{True}
      \end{itemize}
    \end{example}
  \end{columns}
\end{frame}

\begin{frame}
  \frametitle{Exclusive OR}

  \begin{columns}
    \column{.35\textwidth}
    \begin{table}
      \caption{$p \veebar q$}
      \begin{tabular}{|c|c||c|}\hline
        $p$ & $q$ & $p \veebar q$\\\hline\hline
        $T$ & $T$ & $F$          \\\hline
        $T$ & $F$ & $T$          \\\hline
        $F$ & $T$ & $T$          \\\hline
        $F$ & $F$ & $F$          \\\hline
      \end{tabular}
    \end{table}

    \pause
    \column{.65\textwidth}
    \begin{example}
      \begin{itemize}
        \item $p_1 \veebar p_2$: Either the Moon revolves around the Earth or
          elephants can fly.\\
          $T \veebar F$: \emph{True}
      \end{itemize}
    \end{example}
  \end{columns}
\end{frame}

\begin{frame}
  \frametitle{Implication}

  \begin{columns}
    \column{.4\textwidth}
    \begin{table}
      \caption{$p \rightarrow q$}
      \begin{tabular}{|c|c||c|}\hline
        $p$ & $q$ & $p \rightarrow q$\\\hline\hline
        $T$ & $T$ & $T$              \\\hline
        $T$ & $F$ & $F$              \\\hline
        $F$ & $T$ & $T$              \\\hline
        $F$ & $F$ & $T$              \\\hline
      \end{tabular}
    \end{table}

    \pause
    \column{.6\textwidth}
    \begin{itemize}
      \item $p$: \alert{hypothesis}
      \item $q$: \alert{conclusion}

      \item we say:
      \begin{itemize}
        \item if $p$ then $q$
        \item $p$ is sufficient for $q$
        \item $q$ is necessary for $p$
      \end{itemize}

      \pause
      \item $\neg p \vee q$
    \end{itemize}
  \end{columns}
\end{frame}

\begin{frame}
  \frametitle{Implication Examples}

  \begin{example}
    \begin{itemize}
      \item $p_4$: $3<8$, $p_5$: $3<14$, $p_6$: $3<2$
      \item $p_7$: The Sun revolves around the Earth.
    \end{itemize}

    \pause
    \begin{columns}[t]
      \column{.48\textwidth}
        \begin{itemize}
          \item $p_4 \rightarrow p_5$: If 3 is less than 8,\\
            then 3 is less than 14.\\
            $T \rightarrow T$: \emph{True}
          \pause
          \item $p_4 \rightarrow p_6$: If 3 is less than 8,\\
            then 3 is less than 2.\\
            $T \rightarrow F$: \emph{False}
        \end{itemize}

      \pause
      \column{.5\textwidth}
        \begin{itemize}
          \item $p_2 \rightarrow p_1$: If elephants can fly then the Moon
            revolves around the Earth.\\
            $F \rightarrow T$: \emph{True}
          \pause
          \item $p_2 \rightarrow p_7$: If elephants can fly then the Sun
            revolves around the Earth.
            \\
            $F \rightarrow T$: \emph{True}
        \end{itemize}
    \end{columns}
  \end{example}
\end{frame}

\begin{frame}
  \frametitle{Implication Examples}

  \begin{example}
    \begin{columns}
      \column{.6\textwidth}
      \begin{itemize}
        \item "If I weigh over 70 kg, then I will exercise."
        \begin{itemize}
          \item $p$: I weigh over 70 kg.
          \item $q$: I exercise.
        \end{itemize}

        \pause
        \item How to interpret $p \rightarrow q$ ?
      \end{itemize}

      \column{.4\textwidth}
      \begin{table}
        \caption{$p \rightarrow q$}
        \begin{tabular}{|c|c||c|}\hline
          $p$ & $q$ & $p \rightarrow q$\\\hline\hline
          $T$ & $T$ & $T$              \\\hline
          $T$ & $F$ & $F$              \\\hline
          $F$ & $T$ & $T$              \\\hline
          $F$ & $F$ & $T$              \\\hline
        \end{tabular}
      \end{table}
    \end{columns}
  \end{example}
\end{frame}

\begin{frame}
  \frametitle{Biconditional}

  \begin{columns}
    \column{.4\textwidth}
    \begin{table}
      \caption{$p \leftrightarrow q$}
      \begin{tabular}{|c|c||c|}\hline
        $p$ & $q$ & $p \leftrightarrow q$\\\hline\hline
        $T$ & $T$ & $T$                  \\\hline
        $T$ & $F$ & $F$                  \\\hline
        $F$ & $T$ & $F$                  \\\hline
        $F$ & $F$ & $T$                  \\\hline
      \end{tabular}
    \end{table}

    \pause
    \column{.6\textwidth}
    \begin{itemize}
      \item we say:
      \begin{itemize}
        \item $p$ if and only if $q$
        \item $p$ is necessary and sufficient for $q$
      \end{itemize}

      \pause
      \item $(p \rightarrow q) \wedge (q \rightarrow p)$
      \item $\neg (p \veebar q)$
    \end{itemize}
  \end{columns}
\end{frame}

\begin{frame}
  \frametitle{Daily Language Example}

  \begin{example}
    \begin{itemize}
      \item $s$: The child does her homework.
      \item $t$: The child plays a computer game.

      \pause
      \medskip
      \item $s \rightarrow t$\\
        "If you do your homework then you get to play a computer game."
      \item $t \rightarrow s$\\
        "You get to play a computer game only if you do your homework."

      \pause
      \medskip
      \item what the parent really meant: $s \leftrightarrow t$
    \end{itemize}
  \end{example}
\end{frame}

\subsection{Well-Formed Formulas}

\begin{frame}
  \frametitle{Well-Formed Formula}

  \begin{block}{syntax}
    \begin{itemize}
      \item which rules will be used to form compound propositions?
      \item formula that obeys these rules: \alert{well-formed formula} (WFF)
    \end{itemize}
  \end{block}

  \pause
  \begin{block}{semantics}
    \begin{itemize}
      \item \emph{interpretation}: calculating the value of a compound
        proposition by assigning values to its primitive propositions
      \item truth table: all interpretations of a proposition
    \end{itemize}
  \end{block}
\end{frame}

\begin{frame}
  \frametitle{Well-Formed Formula Examples}

  \begin{example}[not a well-formed formula]
    \begin{itemize}
      \item $\vee p$
      \item $p \wedge \neg$
      \item $p \neg \wedge q$
    \end{itemize}
  \end{example}
\end{frame}

\begin{frame}
  \frametitle{Precedence}

  \begin{enumerate}
    \item $\neg$
    \item $\wedge$
    \item $\vee$
    \item $\rightarrow$
    \item $\leftrightarrow$
  \end{enumerate}

  \begin{itemize}
    \item parentheses are used to change precedence
  \end{itemize}
\end{frame}

\begin{frame}
  \frametitle{Precedence Examples}

  \begin{example}
    \begin{itemize}
      \item $s$: Phyllis goes out for a walk.
      \item $t$: The Moon is out.
      \item $u$: It is snowing.
    \end{itemize}

    \medskip
    what is the meaning of the following WFFs?

    \pause
    \begin{itemize}
      \item $t \wedge \neg u \rightarrow s$
      \pause
      \item $t \rightarrow (\neg u \rightarrow s)$
      \pause
      \item $\neg (s \leftrightarrow (u \vee t))$
      \pause
      \item $\neg s \leftrightarrow u \vee t$
    \end{itemize}
  \end{example}
\end{frame}

\begin{frame}
  \frametitle{Formula Types}

  \begin{enumerate}
    \item \emph{tautology}: True for all interpretations
    \item \emph{contradiction}: False for all interpretations
    \item \emph{valid}: True for some interpretations
  \end{enumerate}
\end{frame}

\begin{frame}
  \frametitle{Tautology Example}

  \begin{example}
    \begin{table}
      \caption{$p \wedge (p \rightarrow q) \rightarrow q$}
      \begin{tabular}{|c|c|c|c||c|}\hline
        $p$ & $q$ & $p \rightarrow q$ & $p \wedge (p \rightarrow q)$
            & $p \wedge (p \rightarrow q) \rightarrow q$\\\hline\hline
        $T$ & $T$ & $T$ & $T$ & $T$                     \\\hline
        $T$ & $F$ & $F$ & $F$ & $T$                     \\\hline
        $F$ & $T$ & $T$ & $F$ & $T$                     \\\hline
        $F$ & $F$ & $T$ & $F$ & $T$                     \\\hline
      \end{tabular}
    \end{table}
  \end{example}
\end{frame}

\begin{frame}
  \frametitle{Contradiction Example}

  \begin{example}
    \begin{table}
      \caption{$p \wedge (\neg p \wedge q)$}
      \begin{tabular}{|c|c|c|c||c|}\hline
        $p$ & $q$ & $\neg p$ & $\neg p \wedge q$
            & $p \wedge (\neg p \wedge q)$\\\hline\hline
        $T$ & $T$ & $F$ & $F$ & $F$       \\\hline
        $T$ & $F$ & $F$ & $F$ & $F$       \\\hline
        $F$ & $T$ & $T$ & $T$ & $F$       \\\hline
        $F$ & $F$ & $T$ & $F$ & $F$       \\\hline
      \end{tabular}
    \end{table}
  \end{example}
\end{frame}

\subsection{Metalanguage}

\begin{frame}
  \frametitle{Metalanguage}

  \begin{definition}
    \alert{target language}: language being worked on
  \end{definition}

  \pause
  \begin{definition}
    \alert{metalanguage}: language used when talking about the properties of
      the target language
  \end{definition}

  \pause
  \begin{itemize}
    \item validity, contradiction and tautology are defined in the metalanguage
  \end{itemize}
\end{frame}

\begin{frame}
  \frametitle{Metalanguage Examples}

  \begin{example}[somebody who is learning English]
    \begin{itemize}
      \item target language: English
      \item metalanguage: Turkish
    \end{itemize}
  \end{example}

  \pause
  \begin{example}[Intro. to Sci. and Eng. Comp.]
    \begin{itemize}
      \item target language: C
      \item metalanguage: English
    \end{itemize}
  \end{example}
\end{frame}

\begin{frame}
  \frametitle{Metalogic}

  \begin{itemize}
    \item $P_1,P_2,\dots,P_n \vdash Q$\\
      There is a proof which infers the conclusion $Q$ from the assumptions
      $P_1,P_2,\dots,P_n$.

    \pause
    \medskip
    \item $P_1,P_2,\dots,P_n \vDash Q$\\
      $Q$ must be true if $P_1,P_2,\dots,P_n$ are all true.
  \end{itemize}
\end{frame}

\begin{frame}
  \frametitle{Formal Systems}

  \begin{definition}
    \alert{consistent}: for all well-formed formulas $P$ and $Q$\\
      If $P \vdash Q$ then $P \vDash Q$

    \begin{itemize}
      \item each provable proposition is actually true
    \end{itemize}
  \end{definition}

  \pause
  \begin{definition}
    \alert{complete}: for all well-formed formulas $P$ and $Q$\\
      If $P \vDash Q$ then $P \vdash Q$
    \begin{itemize}
      \item every true proposition can be proven
    \end{itemize}
  \end{definition}
\end{frame}

\begin{frame}
  \frametitle{Gödel's Theorem}

  \begin{itemize}
    \item Propositional logic is consistent and complete.
    \item Predicate logic is both consistent and complete.
  \end{itemize}

  \pause
  \begin{block}{Gödel's Theorem}
    \begin{itemize}
      \item Any logical system that is powerful enough to express ordinary
        arithmetic must be either inconsistent or incomplete!
    \end{itemize}
  \end{block}
\end{frame}

\section{Propositional Calculus}

\subsection{Introduction}

\begin{frame}
  \frametitle{Approaches in Propositional Calculus}

  \begin{enumerate}
    \item semantic approach: \emph{truth tables}
    \begin{itemize}
      \item gets too complicated when the number of primitive statements grow
    \end{itemize}

    \pause
    \item syntactic approach: \emph{rules of inference}
    \begin{itemize}
      \item obtaining new propositions from existing propositions using logical
        implications
    \end{itemize}

    \pause
    \item axiomatic approach: \emph{Boolean algebra}
    \begin{itemize}
      \item substituting equivalent formulas in equations
    \end{itemize}
  \end{enumerate}
\end{frame}

\begin{frame}
  \frametitle{Truth Table Example}

  \begin{example}[$p \rightarrow q$]
    \begin{center}
      \begin{tabular}{|c|c||c|c|c|c|}\hline
        $p$ & $q$ & $p \rightarrow q$ & $\neg q \rightarrow \neg p$ &
                    $q \rightarrow p$ & $\neg p \rightarrow \neg q$\\\hline\hline
        $T$ & $T$ & $T$ & $T$ & $T$ & $T$\\\hline
        $T$ & $F$ & $F$ & $F$ & $T$ & $T$\\\hline
        $F$ & $T$ & $T$ & $T$ & $F$ & $F$\\\hline
        $F$ & $F$ & $T$ & $T$ & $T$ & $T$\\\hline
      \end{tabular}
    \end{center}

    \pause
    \begin{itemize}
      \item \emph{contrapositive}: $\neg q \rightarrow \neg p$

      \pause
      \item \emph{converse}: $q \rightarrow p$

      \pause
      \item \emph{inverse}: $\neg p \rightarrow \neg q$
    \end{itemize}
  \end{example}
\end{frame}

\subsection{Laws of Logic}

\begin{frame}
  \frametitle{Logical Equivalence}

  \begin{definition}
    if $P \leftrightarrow Q$ is a tautology, then $P$ and $Q$ are
    \alert{logically equivalent}:\\
    $P \Leftrightarrow Q$
  \end{definition}
\end{frame}

\begin{frame}
  \frametitle{Logical Equivalence Example}

  \begin{example}
    \begin{itemize}
      \item $\neg p \Leftrightarrow p \rightarrow F$
    \end{itemize}

    \begin{table}
      \caption{$\neg p \leftrightarrow p \rightarrow F$}
      \begin{tabular}{|c|c|c||c|}\hline
        $p$ & $\neg p$ & $p \rightarrow F$
            & $\neg p \leftrightarrow p \rightarrow F$\\\hline\hline
        $T$ & $F$ & $F$ & $T$\\\hline
        $F$ & $T$ & $T$ & $T$\\\hline
      \end{tabular}
    \end{table}
  \end{example}
\end{frame}

\begin{frame}
  \frametitle{Logical Equivalence Example}

  \begin{example}
    \begin{itemize}
      \item $p \rightarrow q \Leftrightarrow \neg p \vee q$
    \end{itemize}

    \begin{table}
      \caption{$(p \rightarrow q) \leftrightarrow (\neg p \vee q)$}
      \begin{tabular}{|c|c|c|c|c||c|}\hline
        $p$ & $q$ & $p \rightarrow q$ & $\neg p$ & $\neg p \vee q$
            & $(p \rightarrow q) \leftrightarrow (\neg p \vee q)$\\\hline\hline
        $T$ & $T$ & $T$ & $F$ & $T$ & $T$\\\hline
        $T$ & $F$ & $F$ & $F$ & $F$ & $T$\\\hline
        $F$ & $T$ & $T$ & $T$ & $T$ & $T$\\\hline
        $F$ & $F$ & $T$ & $T$ & $T$ & $T$\\\hline
      \end{tabular}
    \end{table}
  \end{example}
\end{frame}

\begin{frame}
  \frametitle{Laws of Logic}

  \begin{tabular}{ll}
  \alert{Law of Double Negation (DN)} &\\
    $\neg (\neg p) \Leftrightarrow p$ &\\\\
  \pause
  \alert{Commutative Laws (Co)} &\\
    $p \wedge q \Leftrightarrow q \wedge p$ &
    $p \vee q \Leftrightarrow q \vee p$\\\\
  \pause
  \alert{Associative Laws (As)} &\\
    $(p \wedge q) \wedge r \Leftrightarrow p \wedge (q \wedge r)$ &
    $(p \vee q) \vee r \Leftrightarrow p \vee (q \vee r)$\\\\
  \pause
  \alert{Idempotent Laws (Ip)} &\\
    $p \wedge p \Leftrightarrow p$ &
    $p \vee p \Leftrightarrow p$\\\\
  \pause
  \alert{Inverse Laws (In)} &\\
    $p \wedge \neg p \Leftrightarrow F$ &
    $p \vee \neg p \Leftrightarrow T$
  \end{tabular}
\end{frame}

\begin{frame}
  \frametitle{Laws of Logic}

  \begin{tabular}{ll}
  \alert{Identity Laws (Id)} &\\
    $p \wedge T \Leftrightarrow p$ &
    $p \vee F \Leftrightarrow p$\\\\
  \pause
  \alert{Domination Laws (Do)} &\\
    $p \wedge F \Leftrightarrow F$ &
    $p \vee T \Leftrightarrow T$\\\\
  \pause
  \alert{Distributive Laws (Di)} &\\
    $p \wedge (q \vee r) \Leftrightarrow (p \wedge q) \vee (p \wedge r)$ &
    $p \vee (q \wedge r) \Leftrightarrow (p \vee q) \wedge (p \vee r)$\\\\
  \pause
  \alert{Absorption Laws (Ab)} &\\
    $p \wedge (p \vee q) \Leftrightarrow p$ &
    $p \vee (p \wedge q) \Leftrightarrow p$\\\\
  \pause
  \alert{DeMorgan's Laws (DM)} &\\
    $\neg (p \wedge q) \Leftrightarrow \neg p \vee \neg q$ &
    $\neg (p \vee q) \Leftrightarrow \neg p \wedge \neg q$
  \end{tabular}
\end{frame}

\begin{frame}
  \frametitle{Duality}

  \begin{definition}
    If $s$ contains no logical connectives other than $\wedge$ and $\vee$, then\\
    the \alert{dual} of $s$, denoted $s^d$, is the statement obtained from $s$\\
    by replacing each occurrence of $\wedge$ by $\vee$, and $\vee$ by $\wedge$,\\
    and each occurrence of $T$ by $F$, and $F$ by $T$.
  \end{definition}

  \pause
  \begin{example}[dual proposition]
    \begin{eqnarray*}
      s:   & (p \wedge \neg q) \vee (r \wedge T)\\
      s^d: & (p \vee \neg q) \wedge (r \vee F)
    \end{eqnarray*}
  \end{example}
\end{frame}

\begin{frame}
  \frametitle{Principle of Duality}

  \begin{block}{principle of duality}
    Let $s$ and $t$ be statements that contain no logical connectives\\
    other than $\wedge$ and $\vee$.\\
    If $s \Leftrightarrow t$ then $s^d \Leftrightarrow t^d$.
  \end{block}
\end{frame}

\begin{frame}
  \frametitle{Equivalence Example}

  \begin{example}
    \begin{eqnarray*}
                      & p \rightarrow q           &\\
      \pause
      \Leftrightarrow & \neg p \vee q             &\\
      \pause
      \Leftrightarrow & q \vee \neg p             & Co\\
      \pause
      \Leftrightarrow & \neg \neg q \vee \neg p   & DN\\
      \pause
      \Leftrightarrow & \neg q \rightarrow \neg p &
    \end{eqnarray*}
  \end{example}
\end{frame}

\begin{frame}
  \frametitle{Equivalence Example}

  \begin{example}
    \begin{eqnarray*}
                      & \neg (\neg ((p \vee q) \wedge r) \vee \neg q)      &\\
      \pause
      \Leftrightarrow & \neg \neg ((p \vee q) \wedge r) \wedge \neg \neg q & DM\\
      \pause
      \Leftrightarrow & ((p \vee q) \wedge r) \wedge q                     & DN\\
      \pause
      \Leftrightarrow & (p \vee q) \wedge (r \wedge q)                     & As\\
      \pause
      \Leftrightarrow & (p \vee q) \wedge (q \wedge r)                     & Co\\
      \pause
      \Leftrightarrow & ((p \vee q) \wedge q) \wedge r                     & As\\
      \pause
      \Leftrightarrow & q \wedge r                                         & Ab
    \end{eqnarray*}
  \end{example}
\end{frame}

\subsection{Rules of Inference}

\begin{frame}
  \frametitle{Rules of Inference}

  \begin{definition}
    if $P \rightarrow Q$ is a tautology, then $P$ \alert{logically implies} $Q$:\\
    $P \Rightarrow Q$
  \end{definition}
\end{frame}

\begin{frame}
  \frametitle{Logical Implication Example}

  \begin{example}
    \begin{itemize}
      \item $p \wedge (p \rightarrow q) \Rightarrow q$
    \end{itemize}

    \begin{table}
      \caption{$p \wedge (p \rightarrow q) \rightarrow q$}
      \begin{tabular}{|c|c|c|c||c|}\hline
        $p$ & $q$ & $p \rightarrow q$ & $p \wedge (p \rightarrow q)$
            & $p \wedge (p \rightarrow q) \rightarrow q$\\\hline\hline
        $T$ & $T$ & $T$ & $T$ & $T$\\\hline
        $T$ & $F$ & $F$ & $F$ & $T$\\\hline
        $F$ & $T$ & $T$ & $F$ & $T$\\\hline
        $F$ & $F$ & $T$ & $F$ & $T$\\\hline
      \end{tabular}
    \end{table}
  \end{example}
\end{frame}

\begin{frame}
  \frametitle{Inference}

  \begin{itemize}
    \item establishing the validity of an argument, considering a set of premises
    which have been proven or assumed to be true
  \end{itemize}

  \pause
  \begin{block}{notation}
    \begin{columns}
      \column{.5\textwidth}
      \[
      \frac
        {
          \begin{array}{c}
            p_1\\
            p_2\\
            \dots\\
            p_n
          \end{array}
        }
        {
          \therefore q
        }
      \]

      \column{.5\textwidth}
      $p_1 \wedge p_2 \wedge \cdots \wedge p_n \Rightarrow q$
    \end{columns}
  \end{block}
\end{frame}

\begin{frame}
  \frametitle{Basic Rules}

  \begin{columns}
    \column{.5\textwidth}
    \begin{block}{Identity (ID)}
      \[
      \frac
        {
          \begin{array}{c}
            p
          \end{array}
        }
        {
          \therefore p
        }
      \]
    \end{block}

    \pause
    \column{.5\textwidth}
    \begin{block}{Contradiction (CTR)}
    \[
    \frac
      {
        \begin{array}{c}
          F
        \end{array}
      }
      {
        \therefore p
      }
    \]
    \end{block}
  \end{columns}
\end{frame}

\begin{frame}
  \frametitle{Basic Rules}

  \begin{columns}
    \column{.48\textwidth}
    \begin{block}{Implication Introduction (ImpI)}
      \[
      \frac
        {
          \begin{array}{c}
            p \vdash q
          \end{array}
        }
        {
          \therefore p \rightarrow q
        }
      \]
    \end{block}

    \pause
    \column{.52\textwidth}
    \begin{itemize}
      \item if it can be shown that $q$ is true assuming $p$ is true,\\
        then $p \rightarrow q$ is true\\
        \alert{without assuming $p$ is true}\\
    \end{itemize}
  \end{columns}
\end{frame}

\begin{frame}
  \frametitle{Basic Rules}

  \begin{columns}[t]
    \column{.5\textwidth}
    \begin{block}{AND Introduction (AndI)}
      \[
      \frac
        {
          \begin{array}{c}
            p\\
            q
          \end{array}
        }
        {
          \therefore p \wedge q
        }
      \]
    \end{block}

    \pause
    \column{.5\textwidth}
    \begin{block}{AND Elimination (AndE)}
    \[
    \frac
      {
        \begin{array}{c}
          p \wedge q
        \end{array}
      }
      {
        \therefore p
      }
    \]
    \end{block}
  \end{columns}
\end{frame}

\begin{frame}
  \frametitle{Basic Rules}

  \begin{columns}[t]
    \column{.5\textwidth}
    \begin{block}{OR Introduction (OrI)}
      \[
      \frac
        {
          \begin{array}{c}
            p
          \end{array}
        }
        {
          \therefore p \vee q
        }
      \]
    \end{block}

    \pause
    \column{.5\textwidth}
    \begin{block}{OR Elimination (OrE)}
    \[
    \frac
      {
        \begin{array}{c}
          p \vee q\\
          p \vdash r\\
          q \vdash r
        \end{array}
      }
      {
        \therefore r
      }
    \]
    \end{block}
  \end{columns}
\end{frame}

\begin{frame}
  \frametitle{Basic Rules}

  \begin{columns}[t]
    \column{.5\textwidth}
    \begin{block}{Modus Ponens (ImpE)}
      \[
      \frac
        {
          \begin{array}{c}
            p \rightarrow q\\
            p
          \end{array}
        }
        {
          \therefore q
        }
      \]
    \end{block}

    \pause
    \column{.5\textwidth}
    \begin{block}{Modus Tollens (MT)}
      \[
      \frac
        {
          \begin{array}{c}
            p \rightarrow q\\
            \neg q
          \end{array}
        }
        {
          \therefore \neg p
        }
      \]
    \end{block}
  \end{columns}
\end{frame}

\begin{frame}
  \frametitle{Modus Tollens}

  \begin{example}
    \begin{columns}
      \column{.3\textwidth}
      \[
      \frac
        {
          \begin{array}{c}
            p \rightarrow q\\
            \neg q
          \end{array}
        }
        {
          \therefore \neg p
        }
      \]

      \pause
      \column{.65\textwidth}
      \begin{eqnarray*}
        1. & p \rightarrow q           & Pre\\
        \pause
        2. & \neg q \rightarrow \neg p & 1\\
        \pause
        3. & \neg q                    & Pre\\
        \pause
        4. & \neg p                    & ImpE:2,3\\
      \end{eqnarray*}
    \end{columns}
  \end{example}
\end{frame}

\begin{frame}
  \frametitle{Modus Ponens Example}

  \begin{example}
    \begin{itemize}
      \item Ali will buy a car if he wins the lottery.
      \item Ali has won the lottery.

      \pause
      \medskip
      \item Therefore, Ali will buy a car.
    \end{itemize}
  \end{example}
\end{frame}

\begin{frame}
  \frametitle{Modus Tollens Example}

  \begin{example}
    \begin{itemize}
      \item Ali will buy a car if he wins the lottery.
      \item Ali did not buy a car.

      \pause
      \medskip
      \item Therefore, Ali did not win the lottery.
    \end{itemize}
  \end{example}
\end{frame}

\begin{frame}
  \frametitle{Fallacies}

  \begin{block}{affirming the conclusion}
    \[
    \frac
      {
      \begin{array}{c}
        p \rightarrow q\\
        q
        \end{array}
      }
      {
        \therefore p
      }
    \]
  \end{block}

  \pause
  \begin{itemize}
    \item $(p \rightarrow q) \wedge q \rightarrow p$ is not a tautology:\\
      if $p=F,q=T$: $(F \rightarrow T) \wedge T \rightarrow F$
  \end{itemize}
\end{frame}

\begin{frame}
  \frametitle{Example of Affirming the Conclusion}

  \begin{example}
    \begin{itemize}
      \item If Madonna is the president of the United States,\\
        she is over 35 years old.
      \item Madonna is over 35 years old.

      \pause
      \medskip
      \item Therefore, Madonna is the president of the United States.
    \end{itemize}
  \end{example}
\end{frame}

\begin{frame}
  \frametitle{Fallacies}

  \begin{block}{denying the hypothesis}
    \[
    \frac
      {
        \begin{array}{c}
          p \rightarrow q\\
          \neg p
        \end{array}
      }
      {
        \therefore \neg q
      }
    \]
  \end{block}

  \pause
  \begin{itemize}
    \item $(p \rightarrow q) \wedge \neg p \rightarrow \neg q$ is not a tautology:\\
      if $p=F,q=T$: $(F \rightarrow T) \wedge T \rightarrow F$
  \end{itemize}
\end{frame}

\begin{frame}
  \frametitle{Example of Denying the Hyphothesis}

  \begin{example}
    \begin{itemize}
      \item if $2+3=8$ then $2+4=6$
      \item $2+3 \neq 8$

      \pause
      \medskip
      \item Therefore, $2+4 \neq 6$
    \end{itemize}
  \end{example}
\end{frame}

\begin{frame}
  \frametitle{Disjunctive Syllogism}

  \begin{columns}
    \column{.5\textwidth}
    \begin{block}{Disjunctive Syllogism (DS)}
      \[
      \frac
        {
          \begin{array}{c}
            p \vee q\\
            \neg p
          \end{array}
        }
        {
          \therefore q
        }
      \]
    \end{block}

    \pause
    \column{.5\textwidth}
    \begin{eqnarray*}
      1.   & p \vee q        & Pre\\
      \pause
      2.   & \neg p          & Pre\\
      \pause
      3.   & p \rightarrow F & 2\\
      \pause
      4a1. & p               & Pre!\\
      \pause
      4a2. & F               & ImpE:3,4a1\\
      \pause
      4a.  & q               & CTR:4a2\\
      \pause
      4b1. & q               & Pre!\\
      \pause
      4b.  & q               & ID:4b1\\
      \pause
      5.   & q               & OrE:1,4a,4b
    \end{eqnarray*}
  \end{columns}
\end{frame}

\begin{frame}
  \frametitle{Disjunctive Syllogism Example}

  \begin{example}
    \begin{itemize}
      \item Ali's wallet is either in his pocket or on his desk.
      \item Ali's wallet is not in his pocket.

      \pause
      \medskip
      \item Therefore, Ali's wallet is on his desk.
    \end{itemize}
  \end{example}
\end{frame}

\begin{frame}
  \frametitle{Hypothetical Syllogism}

  \begin{columns}
    \column{.5\textwidth}
    \begin{block}{Hypothetical Syllogism (HS)}
      \[
      \frac
        {
          \begin{array}{c}
            p \rightarrow q\\
            q \rightarrow r
          \end{array}}
        {
          \therefore p \rightarrow r
        }
      \]
    \end{block}

    \pause
    \column{.5\textwidth}
    \begin{eqnarray*}
      1. & p               & Pre!\\
      \pause
      2. & p \rightarrow q & Pre\\
      \pause
      3. & q               & ImpE:2,1\\
      \pause
      4. & q \rightarrow r & Pre\\
      \pause
      5. & r               & ImpE:4,3\\
      \pause
      6. & p \rightarrow r & ImpI:1,5\\
    \end{eqnarray*}
  \end{columns}
\end{frame}

\begin{frame}
  \frametitle{Hypotetical Syllogism Example}

  \begin{example}[Star Trek]
    Spock - to Lieutenant Decker:
    \begin{quote}
      It would be a suicide to attack the enemy ship now. Someone who attempts
      suicide is not psycologically fit to command Enterprise. Therefore, I am
      obliged to relieve you from duty.
    \end{quote}
  \end{example}
\end{frame}

\begin{frame}
  \frametitle{Hypotetical Syllogism Example}

  \begin{example}[Star Trek]
    \begin{itemize}
      \item $p$: Decker attacks the enemy ship.
      \item $q$: Decker attempts suicide.
      \item $r$: Decker is not psycologically fit to command Enterprise.
      \item $s$: Spock relieves Decker from duty.
    \end{itemize}
  \end{example}
\end{frame}

\begin{frame}
  \frametitle{Hypotetical Syllogism Example}

  \begin{example}
    \begin{columns}
      \column{.3\textwidth}
      \[
      \frac
        {
          \begin{array}{c}
            p\\
            p \rightarrow q\\
            q \rightarrow r\\
            r \rightarrow s
          \end{array}
        }
        {
          \therefore s
        }
      \]

      \pause
      \column{.65\textwidth}
      \begin{eqnarray*}
        1. & p \rightarrow q & Pre\\
        \pause
        2. & q \rightarrow r & Pre\\
        \pause
        3. & p \rightarrow r & HS:1,2\\
        \pause
        4. & r \rightarrow s & Pre\\
        \pause
        5. & p \rightarrow s & HS:3,4\\
        \pause
        6. & p               & Pre\\
        \pause
        7. & s               & ImpE:5,6
      \end{eqnarray*}
    \end{columns}
  \end{example}
\end{frame}

\begin{frame}
  \frametitle{Dilemma}

  \begin{columns}[t]
    \column{.5\textwidth}
    \begin{block}{Constructive Dilemma}
      \[
      \frac
        {
          \begin{array}{c}
            p \rightarrow q\\
            r \rightarrow s\\
            p \vee r
          \end{array}}
        {
          \therefore q \vee s
        }
      \]
    \end{block}

    \pause
    \column{.5\textwidth}
    \begin{block}{Destructive Dilemma}
      \[
      \frac
        {
          \begin{array}{c}
            p \rightarrow q\\
            r \rightarrow s\\
            \neg q \vee \neg s
          \end{array}
          }
          {
            \therefore \neg p \vee \neg r
          }
      \]
    \end{block}
  \end{columns}
\end{frame}

\begin{frame}
  \frametitle{Example of Inference}

  \begin{example}
    \begin{columns}[t]
      \column{.25\textwidth}
      \[
      \frac
        {
          \begin{array}{c}
            p \rightarrow r\\
            r \rightarrow s\\
            x \vee \neg s\\
            u \vee \neg x\\
            \neg u
          \end{array}
        }
        {
          \therefore \neg p
        }
      \]

      \pause
      \column{.3\textwidth}
      \begin{eqnarray*}
        1. & u \vee \neg x   & Pre\\
        \pause
        2. & \neg u          & Pre\\
        \pause
        3. & \neg x          & DS:1,2\\
        \pause
        4. & x \vee \neg s   & Pre\\
        \pause
        5. & \neg s          & DS:4,3\\
      \end{eqnarray*}

      \pause
      \column{.45\textwidth}
      \begin{eqnarray*}
        6. & r \rightarrow s & Pre\\
        \pause
        7. & \neg r          & MT:6,5\\
        \pause
        8. & p \rightarrow r & Pre\\
        \pause
        9. & \neg p          & MT:8,7\\
      \end{eqnarray*}
    \end{columns}
  \end{example}
\end{frame}

\begin{frame}
  \frametitle{Example of Inference}

  \begin{example}
    \[
    \frac
      {
        \begin{array}{c}
          (\neg p \vee \neg q) \rightarrow (r \wedge s)\\
          r \rightarrow x\\
          \neg x
        \end{array}
      }
      {
        \therefore p
      }
    \]

    \pause
    \begin{columns}[t]
      \column{.3\textwidth}
      \begin{eqnarray*}
        1. & r \rightarrow x                               & Pre\\
        \pause
        2. & \neg x                                        & Pre\\
        \pause
        3. & \neg r                                        & MT:1,2\\
        \pause
        4. & \neg r \vee \neg s                            & OrI:3\\
        \pause
        5. & \neg (r \wedge s)                             & DM:4
      \end{eqnarray*}

      \pause
      \column{.6\textwidth}
      \begin{eqnarray*}
        6. & (\neg p \vee \neg q) \rightarrow (r \wedge s) & Pre\\
        \pause
        7. & \neg (\neg p \vee \neg q)                     & MT:6,5\\
        \pause
        8. & p \wedge q                                    & DM:7\\
        \pause
        9. & p                                             & AndE:8
      \end{eqnarray*}
    \end{columns}
  \end{example}
\end{frame}

\begin{frame}
  \frametitle{Example of Inference}

  \begin{example}
    \begin{columns}
      \column{.3\textwidth}
      \[
      \frac
        {
          \begin{array}{c}
            p \rightarrow (q \vee r)\\
            s \rightarrow \neg r\\
            q \rightarrow \neg p\\
            p\\
            s
          \end{array}
        }
        {
          \therefore q \wedge \neg q
        }
      \]

      \pause
      \column{.6\textwidth}
      \begin{eqnarray*}
        1. & q \rightarrow \neg p     & Pre\\
       \pause
        2. & p                        & Pre\\
       \pause
        3. & \neg q                   & MT:1,2\\
       \pause
        4. & s                        & Pre\\
       \pause
        5. & s \rightarrow \neg r     & Pre\\
       \pause
        6. & \neg r                   & ImpE:5,4\\
       \pause
        7. & p \rightarrow (q \vee r) & Pre\\
       \pause
        8. & q \vee r                 & ImpE:7,2\\
       \pause
        9. & q                        & DS:8,6\\
       \pause
       10. & q \wedge \neg q          & AndI:9,3
      \end{eqnarray*}
    \end{columns}
  \end{example}
\end{frame}

\begin{frame}
  \frametitle{Example of Inference}

  \begin{example}
    \begin{quote}
      If there is a chance of rain or her red headband is missing, then Lois
      will not mow her lawn. Whenever the temperature is over 20, there is no
      chance for rain. Today the temperature is 22 degrees and Lois is wearing
      her red headband. Therefore, Lois will mow her lawn.
    \end{quote}
  \end{example}
\end{frame}

\begin{frame}
  \frametitle{Example of Inference}

  \begin{example}
    \begin{itemize}
      \item $p$: There is a chance of rain.
      \item $q$: Lois' red headband is lost.
      \item $r$: Lois mows her lawn.
      \item $s$: The temperature is over 20.
    \end{itemize}
  \end{example}
\end{frame}

\begin{frame}
  \frametitle{Example of Inference}

  \begin{example}
    \begin{columns}
      \column{.3\textwidth}
      \[
      \frac
        {
          \begin{array}{c}
            (p \vee q) \rightarrow \neg r\\
            s \rightarrow \neg p\\
            s \wedge \neg q
          \end{array}
        }
        {
          \therefore r
        }
      \]

      \pause
      \column{.65\textwidth}
      \begin{eqnarray*}
        1. & s \wedge \neg q                & Pre\\
        \pause
        2. & s                              & AndE:1\\
        \pause
        3. & s \rightarrow \neg p           & Pre\\
        \pause
        4. & \neg p                         & ImpE:3,2\\
        \pause
        5. & \neg q                         & AndE:1\\
        \pause
        6. & \neg p \wedge \neg q           & AndI:4,5\\
        \pause
        7. & \neg (p \vee q)                & DM:6\\
        \pause
        8. & (p \vee q) \rightarrow \neg r  & Pre\\
        \pause
        9. & ?                              & 7,8
      \end{eqnarray*}
    \end{columns}
  \end{example}
\end{frame}

\section*{References}

\begin{frame}
  \frametitle{References}

  \begin{block}{Required Text: Grimaldi}
    \begin{itemize}
      \item Chapter 2: Fundamentals of Logic
      \begin{itemize}
        \item 2.1. \alert{Basic Connectives and Truth Tables}
        \item 2.2. \alert{Logical Equivalence: The Laws of Logic}\\
        \item 2.3. \alert{Logical Implication: Rules of Inference}
      \end{itemize}
    \end{itemize}
  \end{block}

  \begin{block}{Supplementary Text: O'Donnell, Hall, Page}
    \begin{itemize}
      \item Chapter 6: Propositional Logic
    \end{itemize}
  \end{block}
\end{frame}

\end{document}
